2/3 equiv invs

scripts/memory_model.dfy
@@ -163,46 +163,7 @@ module flat_memory {
     value_256_from_32(x);
     assert flat_read_256(new_flat, ptr) == x;
   }
-
 }
-module heap {
-  import opened flat_memory
-  import opened integers
-
-  datatype entry_t = 
-    | W32(w32: uint32)
-    | B256(b256: seq<uint256>)
-
-  type heap_t = map<int, entry_t>
-
-  datatype mem_t = memory(heap: heap_t, stack: seq<uint32>)
-
-  const STACK_INIT: nat;
-  const STACK_MAX_BYTES: nat := 0x400;
-
-  predicate in_stack_addr_range(addr: int)
-  {
-    STACK_INIT - STACK_MAX_BYTES <= addr <= STACK_INIT
-  }
-
-  predicate valid_stack(mem: mem_t)
-  {
-    && ptr_admissible_32(STACK_INIT)
-    && STACK_MAX_BYTES % 4 == 0
-    && STACK_INIT >= STACK_MAX_BYTES
-    && |mem.stack| == STACK_MAX_BYTES / 4
-  }
-
-  predicate equiv_inv_stack(mem: mem_t, flat: flat_t)
-    requires valid_stack(mem)
-  {
-    && var stack_end := STACK_INIT - STACK_MAX_BYTES;
-    && (forall i | 0 <= i < |mem.stack| ::
-      && var ptr := stack_end + i * 4;
-      && flat_ptr_valid_32(flat, ptr)
-      && mem.stack[i] == flat_read_32(flat, ptr)
-      && ptr !in mem.heap)
-  }
 
   // predicate valid_frames(frames: seq<frame_t>)
   // {
@@ -213,378 +174,447 @@ module heap {
   //     frames[i].fptr <= STACK_INIT - STACK_MAX_SIZE)
   // }
 
-  // valid pointer for W32 heaplet entry
-  predicate heap_ptr_valid_w32(heap: heap_t, base_ptr: nat)
+
+module heap {
+  import opened flat_memory
+  import opened integers
+
+  const STACK_INIT: nat;
+  const STACK_MAX_BYTES: nat := 0x400;
+
+  predicate in_stack_addr_range(addr: int)
   {
-    && ptr_admissible_32(base_ptr)
-    && base_ptr in heap
-    && heap[base_ptr].W32?
-  }
-  // this holds for each W32 heaplet entry
-  predicate equiv_inv_w32(heap: heap_t, flat: flat_t,
-    ptr: nat)
-  {
-    && heap_ptr_valid_w32(heap, ptr)
-    && flat_ptr_valid_32(flat, ptr)
-    && heap[ptr].w32 == flat_read_32(flat, ptr)
-    // disjointness
-    && !in_stack_addr_range(ptr)
+    STACK_INIT - STACK_MAX_BYTES <= addr <= STACK_INIT
   }
 
-  function heap_read_w32(heap: heap_t, ptr: nat): uint32
-    requires heap_ptr_valid_w32(heap, ptr)
-  {
-    heap[ptr].w32
-  }
-
-  function heap_write_w32(heap: heap_t, ptr: nat, value: uint32): heap_t
-    requires heap_ptr_valid_w32(heap, ptr)
-  {
-    heap[ptr := W32(value)]
-  }
-
-  // valid pointer for B256 heaplet entry
-  predicate heap_ptr_valid_b256(heap: heap_t, base_ptr: nat)
-  {
-    && ptr_admissible_256(base_ptr)
-    && base_ptr in heap
-    && heap[base_ptr].B256?
-    && var len := |heap[base_ptr].b256|;
-    //  the buffer is not empty
-    && len != 0
-    // end of buffer is in bound
-    && ptr_admissible_256(buff_index_ptr_b256(base_ptr, len - 1))
-  }
-
-  // iterator for buffer entries
-  datatype iter_b256 = iter_b256_cons(base_ptr: nat, index: nat,
-    ptr: nat, buff: seq<uint256>)
-
-  function buff_index_ptr_b256(ptr: nat, i: nat): nat
+  function heap_b256_index_ptr(ptr: nat, i: nat): nat
   {
     ptr + 32 * i
   }
 
-  predicate iter_b256_inv(iter: iter_b256, heap: heap_t)
-  {
-    var base_ptr := iter.base_ptr;
-    // base_ptr points to a valid buffer
-    && heap_ptr_valid_b256(heap, base_ptr)
-    // ptr is correct
-    && iter.ptr == buff_index_ptr_b256(base_ptr, iter.index)
-    // the view is consistent with heap
-    && heap[base_ptr].b256 == iter.buff
-    // the index is within bound (or at end)
-    && iter.index <= |iter.buff|
-  }
+  // iterator for buffer entries
+  datatype b256_iter = b256_iter_cons(base_ptr: nat, index: nat,
+    ptr: nat, buff: seq<uint256>)
 
-  predicate iter_b256_safe(iter: iter_b256, heap: heap_t)
-  {
-    && iter_b256_inv(iter, heap)
-    // tighter constraint so we can dereference
-    && iter.index < |iter.buff|
-  }
-
-  function iter_b256_load_next(iter: iter_b256, inc: bool): iter_b256
+  function b256_iter_load_next(iter: b256_iter, inc: bool): b256_iter
   {
     iter.(index := if inc then iter.index + 1 else iter.index)
   }
 
-  function iter_b256_store_next(iter: iter_b256, value: uint256, inc: bool): iter_b256
+  function b256_iter_store_next(iter: b256_iter, value: uint256, inc: bool): b256_iter
     requires iter.index < |iter.buff|
   {
       iter.(index := if inc then iter.index + 1 else iter.index)
           .(buff := iter.buff[iter.index := value])
   }
 
-  // this holds for each uint256 in a B256 heaplet entry
-  predicate equiv_inv_256(heap: heap_t, flat: flat_t,
-    base_ptr: nat, i: nat)
-    requires heap_ptr_valid_b256(heap, base_ptr)
-    requires i < |heap[base_ptr].b256|
-  {
-    var ptr := buff_index_ptr_b256(base_ptr, i);
-    // ptr points to some uint256, which has 8 base words uint32
-    && flat_ptr_valid_256(flat, ptr)
-    && flat_read_256(flat, ptr) == heap[base_ptr].b256[i]
-    // disjointness
-    && (i != 0 ==> ptr !in heap)
-    && ptr + 4 !in heap
-    && ptr + 8 !in heap
-    && ptr + 12 !in heap
-    && ptr + 16 !in heap
-    && ptr + 20 !in heap
-    && ptr + 24 !in heap
-    && ptr + 28 !in heap
-    && !in_stack_addr_range(ptr)
-    && !in_stack_addr_range(ptr + 4)
-    && !in_stack_addr_range(ptr + 8)
-    && !in_stack_addr_range(ptr + 12)
-    && !in_stack_addr_range(ptr + 16)
-    && !in_stack_addr_range(ptr + 20)
-    && !in_stack_addr_range(ptr + 24)
-    && !in_stack_addr_range(ptr + 28)
-  }
+  datatype entry_t = 
+    | W32(w32: uint32)
+    | B256(b256: seq<uint256>)
 
-  // this holds for each B256 heaplet entry
-  predicate equiv_inv_b256(heap: heap_t, flat: flat_t,
-    base_ptr: nat)
-    requires heap_ptr_valid_b256(heap, base_ptr)
-  {
-    forall i | 0 <= i < |heap[base_ptr].b256| ::
-      equiv_inv_256(heap, flat, base_ptr, i)
-  }
+  type heap_t = map<int, entry_t>
 
-  function heap_read_b256(heap: heap_t, iter: iter_b256): uint256
-    requires iter_b256_safe(iter, heap)
+  datatype mem_t = memory(heap: heap_t, stack: seq<uint32>)
   {
-    iter.buff[iter.index]
-  }
-
-  function heap_write_b256(heap: heap_t, iter: iter_b256, value: uint256): heap_t
-    requires iter_b256_safe(iter, heap)
-  {
-    var buff := heap[iter.base_ptr].b256;
-    var new_buff := buff[iter.index := value];
-    heap[iter.base_ptr := B256(new_buff)]
-  }
-
-  // the equivalence invariant between heaplet and memory
-  predicate flat_equiv_inv(mem: mem_t, flat: flat_t)
-  {
-    && (forall base_ptr | heap_ptr_valid_b256(mem.heap, base_ptr) ::
-      equiv_inv_b256(mem.heap, flat, base_ptr))
-    && (forall base_ptr | heap_ptr_valid_w32(mem.heap, base_ptr) ::
-      equiv_inv_w32(mem.heap, flat, base_ptr))
-    && valid_stack(mem)
-    && equiv_inv_stack(mem, flat)
-  }
-
-  lemma sub_ptrs_disjoint(mem: mem_t, flat: flat_t, base1: nat, base2: nat)
-    requires flat_equiv_inv(mem, flat)
-    requires heap_ptr_valid_b256(mem.heap, base1)
-    requires heap_ptr_valid_b256(mem.heap, base2)
-    requires base1 != base2
-    ensures forall i, j ::
-      (0 <= i < |mem.heap[base1].b256| && 0 <= j < |mem.heap[base2].b256|)
-        ==> 
-      (buff_index_ptr_b256(base1, i) != buff_index_ptr_b256(base2, j))
-  {
-    var heap := mem.heap;
-    if exists i, j ::
-      && 0 <= i < |heap[base1].b256|
-      && 0 <= j < |heap[base2].b256|
-      && buff_index_ptr_b256(base1, i) == buff_index_ptr_b256(base2, j)
+    predicate stack_valid()
+      requires STACK_MAX_BYTES % 4 == 0
     {
-      var i, j :|
+      && ptr_admissible_32(STACK_INIT)
+      && STACK_INIT >= STACK_MAX_BYTES
+      && |stack| == STACK_MAX_BYTES / 4
+    }
+
+    predicate equiv_inv_stack(flat: flat_t)
+      requires stack_valid()
+    {
+      && var stack_end := STACK_INIT - STACK_MAX_BYTES;
+      && (forall i | 0 <= i < |stack| ::
+        && var ptr := stack_end + i * 4;
+        && flat_ptr_valid_32(flat, ptr)
+        && stack[i] == flat_read_32(flat, ptr)
+        && ptr !in heap)
+    }
+
+    // valid pointer for W32 heaplet entry
+    predicate heap_w32_ptr_valid(base_ptr: nat)
+    {
+      && ptr_admissible_32(base_ptr)
+      && base_ptr in heap
+      && heap[base_ptr].W32?
+    }
+
+    // this holds for each W32 heaplet entry
+    predicate equiv_inv_w32(flat: flat_t, ptr: nat)
+      requires heap_w32_ptr_valid(ptr)
+    {
+      && flat_ptr_valid_32(flat, ptr)
+      && heap[ptr].w32 == flat_read_32(flat, ptr)
+      // disjointness from stack
+      && !in_stack_addr_range(ptr)
+    }
+
+    function heap_w32_read(ptr: nat): uint32
+      requires heap_w32_ptr_valid(ptr)
+    {
+      heap[ptr].w32
+    }
+
+    function heap_w32_write(ptr: nat, value: uint32): mem_t
+      requires heap_w32_ptr_valid(ptr)
+    {
+      this.(heap := heap[ptr := W32(value)])
+    }
+
+    // valid pointer for B256 heaplet entry
+    predicate heap_b256_ptr_valid(base_ptr: nat)
+    {
+      && ptr_admissible_256(base_ptr)
+      && base_ptr in heap
+      && heap[base_ptr].B256?
+      && var len := |heap[base_ptr].b256|;
+      //  the buffer is not empty
+      && len != 0
+      // end of buffer is in bound
+      && ptr_admissible_256(heap_b256_index_ptr(base_ptr, len - 1))
+    }
+
+    predicate b256_iter_inv(iter: b256_iter)
+    {
+      var base_ptr := iter.base_ptr;
+      // base_ptr points to a valid buffer
+      && heap_b256_ptr_valid(base_ptr)
+      // ptr is correct
+      && iter.ptr == heap_b256_index_ptr(base_ptr, iter.index)
+      // the view is consistent with heap
+      && heap[base_ptr].b256 == iter.buff
+      // the index is within bound (or at end)
+      && iter.index <= |iter.buff|
+    }
+
+    predicate b256_iter_safe(iter: b256_iter)
+    {
+      && b256_iter_inv(iter)
+      // tighter constraint so we can dereference
+      && iter.index < |iter.buff|
+    }
+
+    // this holds for each uint256 in a B256 heaplet entry
+    predicate heap_256_equiv_inv(flat: flat_t, base_ptr: nat, i: nat)
+      requires heap_b256_ptr_valid(base_ptr)
+      requires i < |heap[base_ptr].b256|
+    {
+      var ptr := heap_b256_index_ptr(base_ptr, i);
+      // ptr points to some uint256, which has 8 base words uint32
+      && flat_ptr_valid_256(flat, ptr)
+      && flat_read_256(flat, ptr) == heap[base_ptr].b256[i]
+      // disjointness
+      && (i != 0 ==> ptr !in heap)
+      && ptr + 4 !in heap
+      && ptr + 8 !in heap
+      && ptr + 12 !in heap
+      && ptr + 16 !in heap
+      && ptr + 20 !in heap
+      && ptr + 24 !in heap
+      && ptr + 28 !in heap
+      && !in_stack_addr_range(ptr)
+      && !in_stack_addr_range(ptr + 4)
+      && !in_stack_addr_range(ptr + 8)
+      && !in_stack_addr_range(ptr + 12)
+      && !in_stack_addr_range(ptr + 16)
+      && !in_stack_addr_range(ptr + 20)
+      && !in_stack_addr_range(ptr + 24)
+      && !in_stack_addr_range(ptr + 28)
+    }
+
+    // this holds for each B256 heaplet entry
+    predicate heap_b256_equiv_inv(flat: flat_t, base_ptr: nat)
+      requires heap_b256_ptr_valid(base_ptr)
+    {
+      forall i | 0 <= i < |heap[base_ptr].b256| ::
+        heap_256_equiv_inv(flat, base_ptr, i)
+    }
+
+    function heap_read_b256(iter: b256_iter): uint256
+      requires b256_iter_safe(iter)
+    {
+      iter.buff[iter.index]
+    }
+
+    function heap_b256_write(iter: b256_iter, value: uint256): mem_t
+      requires b256_iter_safe(iter)
+    {
+      var buff := heap[iter.base_ptr].b256;
+      var new_buff := buff[iter.index := value];
+      this.(heap := heap[iter.base_ptr := B256(new_buff)])
+    }
+
+    // the equivalence invariant between heaplet and memory
+    predicate flat_equiv_inv(flat: flat_t)
+    {
+      && (forall base_ptr | heap_b256_ptr_valid(base_ptr) ::
+        heap_b256_equiv_inv(flat, base_ptr))
+      && (forall base_ptr | heap_w32_ptr_valid(base_ptr) ::
+        equiv_inv_w32(flat, base_ptr))
+      && stack_valid()
+      && equiv_inv_stack(flat)
+    }
+
+    lemma sub_ptrs_disjoint(flat: flat_t, base1: nat, base2: nat)
+      requires flat_equiv_inv(flat)
+      requires heap_b256_ptr_valid(base1)
+      requires heap_b256_ptr_valid(base2)
+      requires base1 != base2
+      ensures forall i, j ::
+        (0 <= i < |heap[base1].b256| && 0 <= j < |heap[base2].b256|)
+          ==> 
+        (heap_b256_index_ptr(base1, i) != heap_b256_index_ptr(base2, j))
+    {
+      var heap := heap;
+      if exists i, j ::
         && 0 <= i < |heap[base1].b256|
         && 0 <= j < |heap[base2].b256|
-        && buff_index_ptr_b256(base1, i) == buff_index_ptr_b256(base2, j);
-      assert base1 + 32 * i == base2 + 32 * j;
-      var buff1 := heap[base1].b256;
-      var buff2 := heap[base2].b256;
+        && heap_b256_index_ptr(base1, i) == heap_b256_index_ptr(base2, j)
+      {
+        var i, j :|
+          && 0 <= i < |heap[base1].b256|
+          && 0 <= j < |heap[base2].b256|
+          && heap_b256_index_ptr(base1, i) == heap_b256_index_ptr(base2, j);
+        assert base1 + 32 * i == base2 + 32 * j;
+        var buff1 := heap[base1].b256;
+        var buff2 := heap[base2].b256;
 
-      if base1 > base2 {
-        assert equiv_inv_b256(heap, flat, base2);
-        var k := j - i;
-        assert base1 == buff_index_ptr_b256(base2, k);
-        assert 0 <= k < |buff2|;
-        assert equiv_inv_256(heap, flat, base2, k);
-        assert base1 !in heap;
-        assert false;
+        if base1 > base2 {
+          assert heap_b256_equiv_inv(flat, base2);
+          var k := j - i;
+          assert base1 == heap_b256_index_ptr(base2, k);
+          assert 0 <= k < |buff2|;
+          assert heap_256_equiv_inv(flat, base2, k);
+          assert base1 !in heap;
+          assert false;
+        } else {
+          assert heap_b256_equiv_inv(flat, base1);
+          var k := i - j;
+          assert base2 == heap_b256_index_ptr(base1, k);
+          assert 0 <= k < |buff1|;
+          assert heap_256_equiv_inv(flat, base1, k);
+          assert base2 !in heap;
+          assert false;
+        }
+      }
+    }
+
+    lemma heap_b256_write_preserves_b256_inv(
+      new_mem: mem_t,
+      flat: flat_t, new_flat: flat_t,
+      iter: b256_iter, value: uint256,
+      other_ptr: nat)
+
+      requires flat_equiv_inv(flat)
+      requires b256_iter_safe(iter)
+      requires heap_b256_ptr_valid(other_ptr)
+      requires heap_b256_equiv_inv(flat, other_ptr)
+      requires new_mem == heap_b256_write(iter, value)
+      requires new_flat == flat_write_256(flat, iter.ptr, value)
+
+      ensures new_mem.heap_b256_equiv_inv(new_flat, other_ptr)
+    {
+      var base_ptr, j := iter.base_ptr, iter.index;
+      var buff := heap[other_ptr].b256;
+      var len := |buff|;
+
+      if other_ptr == base_ptr {
+        forall i | 0 <= i < len
+          ensures new_mem.heap_256_equiv_inv(new_flat, base_ptr, i)
+        {
+          assert heap_256_equiv_inv(flat, base_ptr, i);
+          if i == j {
+            value_256_from_32(value);
+            assert new_mem.heap_256_equiv_inv(new_flat, base_ptr, i);
+          }
+        }
       } else {
-        assert equiv_inv_b256(heap, flat, base1);
-        var k := i - j;
-        assert base2 == buff_index_ptr_b256(base1, k);
-        assert 0 <= k < |buff1|;
-        assert equiv_inv_256(heap, flat, base1, k);
-        assert base2 !in heap;
-        assert false;
-      }
-    }
-  }
-
-  lemma heap_write_b256_preserves_b256_inv(
-    mem: mem_t, new_heap: heap_t,
-    iter: iter_b256, 
-    flat: flat_t, new_flat: flat_t,
-    value: uint256,
-    other_ptr: nat)
-
-    requires flat_equiv_inv(mem, flat)
-    requires iter_b256_safe(iter, mem.heap)
-    requires heap_ptr_valid_b256(mem.heap, other_ptr)
-    requires equiv_inv_b256(mem.heap, flat, other_ptr)
-    requires new_heap == heap_write_b256(mem.heap, iter, value)
-    requires new_flat == flat_write_256(flat, iter.ptr, value)
-
-    ensures equiv_inv_b256(new_heap, new_flat, other_ptr)
-  {
-    var heap := mem.heap;
-    var base_ptr, j := iter.base_ptr, iter.index;
-    var buff := heap[other_ptr].b256;
-    var new_buff := new_heap[other_ptr].b256;
-    var len := |buff|;
-
-    if other_ptr == base_ptr {
-      forall i | 0 <= i < len
-        ensures equiv_inv_256(new_heap, new_flat, base_ptr, i)
-      {
-        assert equiv_inv_256(heap, flat, base_ptr, i);
-        if i == j {
-          value_256_from_32(value);
-          assert equiv_inv_256(new_heap, new_flat, base_ptr, i);
+        forall i | 0 <= i < len
+          ensures new_mem.heap_256_equiv_inv(new_flat, other_ptr, i)
+        {
+          assert heap_256_equiv_inv(flat, other_ptr, i);
+          var ptr := heap_b256_index_ptr(other_ptr, i);
+          assert flat_ptr_valid_256(new_flat, ptr);
+          assert ptr != iter.ptr by {
+            sub_ptrs_disjoint(flat, other_ptr, base_ptr);
+          }
+          assert flat_read_256(new_flat, ptr) == buff[i];
         }
       }
-    } else {
-      forall i | 0 <= i < len
-        ensures equiv_inv_256(new_heap, new_flat, other_ptr, i)
+      assert heap_b256_equiv_inv(flat, other_ptr);
+    }
+
+    lemma heap_b256_write_preserves_stack_inv(
+      new_mem: mem_t,
+      flat: flat_t, new_flat: flat_t,
+      iter: b256_iter, value: uint256)
+
+      requires flat_equiv_inv(flat)
+      requires b256_iter_safe(iter)
+
+      requires new_mem == heap_b256_write(iter, value)
+      requires new_flat == flat_write_256(flat, iter.ptr, value)
+
+      ensures new_mem.equiv_inv_stack(new_flat)
+    {
+      var stack_end := STACK_INIT - STACK_MAX_BYTES;
+
+      forall i | 0 <= i < |new_mem.stack|
+        ensures
+          && var ptr := stack_end + i * 4;
+          && flat_ptr_valid_32(new_flat, ptr)
+          && new_mem.stack[i] == flat_read_32(new_flat, ptr)
+          && ptr !in new_mem.heap
       {
-        assert equiv_inv_256(heap, flat, other_ptr, i);
-        var ptr := buff_index_ptr_b256(other_ptr, i);
-        assert flat_ptr_valid_256(new_flat, ptr);
-        assert ptr != iter.ptr by {
-          sub_ptrs_disjoint(mem, flat, other_ptr, base_ptr);
+        var ptr := stack_end + i * 4;
+        assert flat_ptr_valid_32(new_flat, ptr);
+
+        if flat_read_32(new_flat, ptr) != flat_read_32(flat, ptr) {
+          // this pointer can't be in stack range
+          assert heap_256_equiv_inv(flat, iter.base_ptr, iter.index);
+          assert false;
         }
-        assert flat_read_256(new_flat, ptr) == buff[i];
       }
     }
-    assert equiv_inv_b256(heap, flat, other_ptr);
+
+    lemma heap_b256_write_preserves_w32_inv(
+      new_mem: mem_t,
+      flat: flat_t, new_flat: flat_t,
+      iter: b256_iter, value: uint256,
+      other_ptr: nat)
+
+      requires flat_equiv_inv(flat)
+      requires b256_iter_safe(iter)
+      requires heap_w32_ptr_valid(other_ptr)
+      requires new_mem== heap_b256_write(iter, value)
+      requires new_flat == flat_write_256(flat, iter.ptr, value)
+
+      ensures new_mem.equiv_inv_w32(new_flat, other_ptr)
+      {
+        if flat[other_ptr] != new_flat[other_ptr] {
+          assert heap_256_equiv_inv(flat, iter.base_ptr, iter.index);
+          assert false;
+        }
+      }
+
+    lemma heap_b256_write_preverses_flat_equiv(
+      new_mem: mem_t,
+      flat: flat_t, new_flat: flat_t,
+      iter: b256_iter, value: uint256)
+
+      requires flat_equiv_inv(flat)
+      requires b256_iter_safe(iter)
+      requires new_mem == heap_b256_write(iter, value)
+      requires new_flat == flat_write_256(flat, iter.ptr, value)
+
+      ensures new_mem.flat_equiv_inv(new_flat)
+    {
+      forall base_ptr | new_mem.heap_b256_ptr_valid(base_ptr)
+        ensures new_mem.heap_b256_equiv_inv(new_flat, base_ptr)
+      {
+        heap_b256_write_preserves_b256_inv(new_mem,
+          flat, new_flat, iter, value, base_ptr);
+      }
+      forall base_ptr | new_mem.heap_w32_ptr_valid(base_ptr)
+        ensures new_mem.equiv_inv_w32(new_flat, base_ptr)
+      {
+        heap_b256_write_preserves_w32_inv(new_mem,
+          flat, new_flat, iter, value, base_ptr);
+      }
+
+      heap_b256_write_preserves_stack_inv(new_mem,
+        flat, new_flat, iter, value);
+    }
+
+    lemma heap_w32_write_preserves_b256_inv(
+      new_mem: mem_t,
+      flat: flat_t, new_flat: flat_t,
+      value: uint32,
+      write_ptr: nat, other_ptr: nat)
+
+    requires flat_equiv_inv(flat)
+    requires heap_w32_ptr_valid(write_ptr)
+    requires heap_b256_ptr_valid(other_ptr)
+    requires new_mem == heap_w32_write(write_ptr, value)
+    requires new_flat == flat_write_32(flat, write_ptr, value)
+
+    ensures new_mem.heap_b256_equiv_inv(new_flat, other_ptr)
+    {
+      assert heap_b256_equiv_inv(flat, other_ptr);
+      var buff := heap[other_ptr].b256;
+      forall i | 0 <= i < |buff| 
+        ensures new_mem.heap_256_equiv_inv(new_flat, other_ptr, i)
+      {
+        assert heap_256_equiv_inv(flat, other_ptr, i);
+      }
+    }
+
+    lemma heap_w32_write_preserves_w32_inv(
+      new_mem: mem_t,
+      flat: flat_t, new_flat: flat_t,
+      value: uint32,
+      write_ptr: nat, other_ptr: nat)
+
+      requires flat_equiv_inv(flat)
+      requires heap_w32_ptr_valid(write_ptr)
+      requires heap_w32_ptr_valid(other_ptr)
+      requires new_mem == heap_w32_write(write_ptr, value)
+      requires new_flat == flat_write_32(flat, write_ptr, value)
+
+      ensures new_mem.equiv_inv_w32(new_flat, other_ptr)
+    {
+      if other_ptr == write_ptr {
+        value_32_from_32(value);
+      }
+    }
+
+    lemma heap_w32_write_preserves_stack_inv(
+      new_mem: mem_t,
+      flat: flat_t, new_flat: flat_t,
+      value: uint32,
+      write_ptr: nat)
+
+      requires flat_equiv_inv(flat)
+      requires heap_w32_ptr_valid(write_ptr)
+      requires new_mem == heap_w32_write(write_ptr, value)
+      requires new_flat == flat_write_32(flat, write_ptr, value)
+
+      ensures new_mem.equiv_inv_stack(new_flat)
+    {
+    }
+
+    lemma heap_w32_write_preverses_flat_equiv(
+      new_mem: mem_t,
+      flat: flat_t, new_flat: flat_t,
+      value: uint32,
+      write_ptr: nat)
+
+      requires flat_equiv_inv(flat)
+      requires heap_w32_ptr_valid(write_ptr)
+      requires new_mem == heap_w32_write(write_ptr, value)
+      requires new_flat == flat_write_32(flat, write_ptr, value)
+
+      ensures new_mem.flat_equiv_inv(new_flat)
+    {
+      forall base_ptr | new_mem.heap_b256_ptr_valid(base_ptr)
+        ensures new_mem.heap_b256_equiv_inv(new_flat, base_ptr)
+      {
+        heap_w32_write_preserves_b256_inv(new_mem,
+          flat, new_flat, value, write_ptr, base_ptr);
+      }
+      forall base_ptr | new_mem.heap_w32_ptr_valid(base_ptr)
+        ensures new_mem.equiv_inv_w32(new_flat, base_ptr)
+      {
+        heap_w32_write_preserves_w32_inv(new_mem,
+          flat, new_flat, value, write_ptr, base_ptr);
+      }
+
+      heap_w32_write_preserves_stack_inv(new_mem,
+        flat, new_flat, value, write_ptr);
+    }
   }
-
-  lemma heap_write_b256_preserves_stack_inv(
-    mem: mem_t, new_heap: heap_t,
-    iter: iter_b256, 
-    flat: flat_t, new_flat: flat_t,
-    value: uint256)
-
-    requires flat_equiv_inv(mem, flat)
-    requires iter_b256_safe(iter, mem.heap)
-
-    requires new_heap == heap_write_b256(mem.heap, iter, value)
-    requires new_flat == flat_write_256(flat, iter.ptr, value)
-
-
-  // lemma heap_write_b256_preserves_w32_inv(
-  //   heap: heap_t, new_heap: heap_t,
-  //   iter: iter_b256, 
-  //   flat: flat_t, new_flat: flat_t,
-  //   value: uint256,
-  //   other_ptr: nat)
-
-  //   requires flat_equiv_inv(heap, flat)
-  //   requires iter_b256_safe(iter, heap)
-  //   requires equiv_inv_w32(heap, flat, other_ptr)
-  //   requires new_heap == heap_write_b256(heap, iter, value)
-  //   requires new_flat == flat_write_256(flat, iter.ptr, value)
-
-  //   ensures equiv_inv_w32(new_heap, new_flat, other_ptr)
-  //   {
-  //     assert heap[other_ptr] == new_heap[other_ptr];
-  //     if flat[other_ptr] != new_flat[other_ptr] {
-        
-  //       assert equiv_inv_256(heap, flat, iter.base_ptr, iter.index);
-  //       assert false;
-  //     }
-  //   }
-
-  // lemma heap_write_b256_preverses_flat_equiv(
-  //   heap: heap_t, new_heap: heap_t,
-  //   iter: iter_b256, 
-  //   flat: flat_t, new_flat: flat_t,
-  //   value: uint256)
-
-  //   requires flat_equiv_inv(heap, flat)
-  //   requires iter_b256_safe(iter, heap)
-  //   requires new_heap == heap_write_b256(heap, iter, value)
-  //   requires new_flat == flat_write_256(flat, iter.ptr, value)
-
-  //   ensures flat_equiv_inv(new_heap, new_flat)
-  // {
-  //   forall base_ptr | heap_ptr_valid_b256(new_heap, base_ptr)
-  //     ensures equiv_inv_b256(new_heap, new_flat, base_ptr)
-  //   {
-  //     heap_write_b256_preserves_b256_inv(heap, new_heap,
-  //       iter, flat, new_flat, value, base_ptr);
-  //   }
-  //   forall base_ptr | heap_ptr_valid_w32(new_heap, base_ptr)
-  //     ensures equiv_inv_w32(new_heap, new_flat, base_ptr)
-  //   {
-  //     heap_write_b256_preserves_w32_inv(heap, new_heap,
-  //       iter, flat, new_flat, value, base_ptr);
-  //   }
-  // }
-
-  // lemma heap_write_w32_preserves_b256_inv(
-  //   heap: heap_t, new_heap: heap_t,
-  //   flat: flat_t, new_flat: flat_t,
-  //   value: uint32,
-  //   write_ptr: nat,
-  //   other_ptr: nat)
-
-  //   requires flat_equiv_inv(heap, flat)
-  //   requires equiv_inv_w32(heap, flat, write_ptr)
-  //   requires equiv_inv_b256(heap, flat, other_ptr)
-  //   requires new_heap == heap_write_w32(heap, write_ptr, value)
-  //   requires new_flat == flat_write_32(flat, write_ptr, value)
-
-  //   ensures equiv_inv_b256(new_heap, new_flat, other_ptr)
-  // {
-  //   assert heap[other_ptr] == new_heap[other_ptr];
-  //   var buff := heap[other_ptr].b256;
-
-  //   forall i | 0 <= i < |buff| 
-  //     ensures equiv_inv_256(new_heap, new_flat, other_ptr, i)
-  //   {
-  //     assert equiv_inv_256(heap, flat, other_ptr, i);
-  //   }
-  // }
-
-  // lemma heap_write_w32_preserves_w32_inv(
-  //   heap: heap_t, new_heap: heap_t,
-  //   flat: flat_t, new_flat: flat_t,
-  //   value: uint32,
-  //   write_ptr: nat,
-  //   other_ptr: nat)
-
-  //   requires flat_equiv_inv(heap, flat)
-  //   requires equiv_inv_w32(heap, flat, write_ptr)
-  //   requires equiv_inv_w32(heap, flat, other_ptr)
-  //   requires new_heap == heap_write_w32(heap, write_ptr, value)
-  //   requires new_flat == flat_write_32(flat, write_ptr, value)
-
-  //   ensures equiv_inv_w32(new_heap, new_flat, other_ptr)
-  // {
-  //   if other_ptr == write_ptr {
-  //     value_32_from_32(value);
-  //   }
-  // }
-
-  // lemma heap_write_w32_preverses_flat_equiv(
-  //   heap: heap_t, new_heap: heap_t,
-  //   flat: flat_t, new_flat: flat_t,
-  //   write_ptr: nat,
-  //   value: uint32)
-
-  //   requires flat_equiv_inv(heap, flat)
-  //   requires equiv_inv_w32(heap, flat, write_ptr)
-  //   requires new_heap == heap_write_w32(heap, write_ptr, value)
-  //   requires new_flat == flat_write_32(flat, write_ptr, value)
-
-  //   ensures flat_equiv_inv(new_heap, new_flat)
-  // {
-  //   forall base_ptr | heap_ptr_valid_b256(new_heap, base_ptr)
-  //     ensures equiv_inv_b256(new_heap, new_flat, base_ptr)
-  //   {
-  //     heap_write_w32_preserves_b256_inv(heap, new_heap,
-  //       flat, new_flat, value, write_ptr, base_ptr);
-  //   }
-  //   forall base_ptr | heap_ptr_valid_w32(new_heap, base_ptr)
-  //     ensures equiv_inv_w32(new_heap, new_flat, base_ptr)
-  //   {
-  //     heap_write_w32_preserves_w32_inv(heap, new_heap,
-  //       flat, new_flat, value, write_ptr, base_ptr);
-  //   }
-  // }
-
 }
